Prove return to main location correct

Compilation.thy
@@ -302,7 +302,7 @@ lemma last_ies_empty:
       and dnz: "durations_positive"
       and fpl:  "finite_plan"
   shows "IES (time_index (length htpl - 1)) = {}" (is "IES ?te = {}")
-proof -
+proof -   
   have "a \<notin> IES ?te" for a
   proof (rule notI)
     assume a: "a \<in> IES ?te"
@@ -1735,7 +1735,6 @@ proof -
   qed 
   thus ?thesis unfolding prop_model_def by blast
 qed
-term limited_snap_action_set
 
 lemma conditional_application_is_application:
   assumes "\<forall>a b. a \<in> S \<and> b \<in> S \<and> a \<noteq> b \<longrightarrow> \<not>(mutex_snap_action a b)"
@@ -2471,12 +2470,198 @@ proof -
       apply -
       apply (subst (asm) act_pred[symmetric])+
       unfolding exec_model_def by blast
+  qed
+
+abbreviation "Inv \<equiv> invs_at plan_inv_seq"
+
+lemma invs_of_active_actions: 
+  assumes pap: plan_actions_in_problem
+      and nso: no_self_overlap
+      and dp: durations_positive 
+  shows
+  "Inv t = \<Union>(over_all ` (ES t))"
+proof (rule equalityI; rule subsetI)
+  fix x
+  assume "x \<in> Inv t"
+  then obtain a t' d where
+    x: "x \<in> over_all a"
+    "(a, t', d) \<in> ran \<pi>" 
+    "t' < t \<and> t \<le> t' + d" unfolding invs_at_def plan_inv_seq_def by blast
+  hence t': "(t', at_start a) \<in> plan_happ_seq \<and> t' < t" unfolding plan_happ_seq_def by auto 
+  moreover
+  from x
+  have a_in_acts: "a \<in> actions" using pap unfolding plan_actions_in_problem_def by blast
+  have "\<not> (\<exists>s. (s, at_end a) \<in> plan_happ_seq \<and> t' \<le> s \<and> s < t)"
+  proof (rule notI)
+    assume "\<exists>s. (s, at_end a) \<in> plan_happ_seq \<and> t' \<le> s \<and> s < t"
+    then obtain s where
+      s: "(s, at_end a) \<in> plan_happ_seq"
+      "t' \<le> s" "s < t" by blast
+    then obtain s' d' where
+      s': "s = s' + d'"
+      "(a, s', d') \<in> ran \<pi>" using at_end_in_happ_seqE a_in_acts pap nso dp by blast
+    hence "(s', at_start a) \<in> plan_happ_seq" unfolding plan_happ_seq_def by blast
+    show False
+    proof (cases "s' < t'")
+      case True
+      with s(2)[simplified s'(1)]
+      show ?thesis using nso[THEN no_self_overlap_spec, OF s'(2) x(2)] by fastforce
+    next
+      case False
+      from s s'
+      have "s' + d' < t" by simp
+      moreover
+      from x
+      have "t \<le> t' + d" by simp
+      ultimately
+      have "s' + d' < t' + d" by simp
+      moreover
+      from dp[simplified durations_positive_def] s'(2)
+      have "0 < d'" by simp
+      ultimately
+      have "s' < t' + d" by (meson less_add_same_cancel1 order_less_trans)
+      moreover
+      from False
+      have "t' = s' \<longrightarrow> d' \<noteq> d" using s x t' s' by auto
+      ultimately
+      show ?thesis using nso[THEN no_self_overlap_spec, OF x(2) s'(2)] False by fastforce
+    qed
+  qed
+  ultimately
+  have "a \<in> ES t" unfolding exec_state_sequence_def using a_in_acts by blast
+  with x
+  show "x \<in> \<Union> (over_all ` ES t)" by blast
+next 
+  fix x
+  assume "x \<in> \<Union> (over_all ` ES t)"
+  then obtain t' a where
+    x: "x \<in> over_all a"
+    "a \<in> actions"
+    "(t', at_start a) \<in> plan_happ_seq"
+    "t' < t"
+    "\<not>(\<exists>s. (s, at_end a) \<in> plan_happ_seq \<and> t' \<le> s \<and> s < t)"
+    unfolding exec_state_sequence_def by force
+  then obtain d where
+    a: "(a, t', d) \<in> ran \<pi>" using at_start_in_happ_seqE nso dp pap by blast
+  have "t' + d \<ge> t" 
+  proof (rule ccontr)
+    assume "\<not> t \<le> t' + d"
+    hence "t' + d < t" by simp
+    moreover
+    have "(t' + d, at_end a) \<in> plan_happ_seq" using a unfolding plan_happ_seq_def by blast
+    moreover
+    have "t' < t' + d" using dp[simplified durations_positive_def] a by auto
+    ultimately
+    show False using x(5) by simp
+  qed
+  with a x
+  show "x \<in> Inv t" unfolding invs_at_def plan_inv_seq_def by auto
+qed
+
+lemma return_to_main:
+  assumes prop_model:   "prop_model W (MS (Suc l))"
+  and exec_model:       "exec_model W (IES (time_index l))"
+  and start_times_corr: "\<forall>a \<in> actions. W (StartDur a) = exec_time' (at_start a) (time_index l)"
+  and end_times_corr:   "\<forall>a \<in> actions. W (EndDur a) = exec_time' (at_end a) (time_index l)"
+  and stop:             "W Stop = 0"
+  and l:                "l < length htpl"
+  and vss: "valid_state_sequence MS"
+  and pap: plan_actions_in_problem
+  and nso: no_self_overlap
+  and dp: durations_positive 
+  and fp: finite_plan
+    shows "\<T> \<turnstile> \<langle>Execution (at_end (act M)), W\<rangle> \<rightarrow>* \<langle>Main, W(Delta:=0)\<rangle>"
+proof -
+  have over_all: "W \<turnstile> action_over_all a" if a_in_actions: "a \<in> actions" for a 
+  proof (cases "a \<in> IES (time_index l)")
+    case True
+    with exec_model that
+    have running: "W (Running a) = 1" unfolding exec_model_def by blast
+    
+    
+    have "W p = 1" if "p \<in> set (map PropClock (prop_list (over_all a)))" for p
+    proof -
+      from that obtain pr where
+        pr: "pr \<in> set (prop_list (over_all a))"
+         "p = PropClock pr" by auto
+      
+      have oap: "over_all a \<subseteq> props" using wf_acts \<open>a \<in> actions\<close> by auto
+      hence "set (prop_list (over_all a)) = over_all a" using set_prop_list by auto
+      with pr
+      have pr_in_a_invs: "pr \<in> over_all a" by simp
+      moreover
+      from True last_ies_empty pap dp fp
+      have sl: "Suc l < length htpl" by (metis Suc_lessI diff_Suc_1 empty_iff l)
+      with inc_es_is_next_es fp True
+      have "a \<in> ES (time_index (Suc l))" by blast
+      ultimately 
+      have "pr \<in> Inv (time_index (Suc l))" using invs_of_active_actions pap nso dp by blast
+      moreover
+      from vss
+      have "Inv (time_index (Suc l)) \<subseteq> MS (Suc l)" unfolding valid_state_sequence_def using sl by (auto simp: Let_def)
+      ultimately
+      have "pr \<in> MS (Suc l)" by blast 
+      moreover
+      from pr_in_a_invs a_in_actions
+      have "pr \<in> props" using wf_acts by auto
+      ultimately
+      have "W (PropClock pr) = 1" using prop_model unfolding prop_model_def by simp
+      thus ?thesis using pr by simp
+    qed
+    with running
+    have "list_all (\<lambda>p. W \<turnstile> CLE (Running a) p 0) (over_all_clocks a)"
+      unfolding over_all_clocks_def
+      using list_all_iff by force
+    then show ?thesis unfolding action_over_all_def AND_ALL_iff list_all_iff by simp
+  next
+    case False
+    with exec_model that
+    have not_running: "W (Running a) = 0" unfolding exec_model_def by blast
+    moreover
+    from prop_model
+    have prop_cases: "\<forall>p \<in> props. W (PropClock p) = 0 \<or> W (PropClock p) = 1" unfolding prop_model_def by blast
+    have oap: "over_all a \<subseteq> props" using wf_acts that by auto
+    hence "set (prop_list (over_all a)) = over_all a" using set_prop_list by auto
+    with oap prop_cases
+    have "\<forall>p \<in> set (prop_list (over_all a)). W (PropClock p) = 0 \<or> W (PropClock p) = 1" by blast
+    hence "\<forall>p \<in> set (map PropClock (prop_list (over_all a))). W p = 0 \<or> W p = 1" by simp
+    with not_running
+    have "list_all (\<lambda>p. W \<turnstile> CLE (Running a) p 0) (over_all_clocks a)"
+      unfolding over_all_clocks_def list_all_iff
+      apply -
+      apply (rule ballI)
+      subgoal for p
+        apply (drule bspec[where x = p])
+         apply assumption
+        apply (erule disjE) 
+        by auto
+      done
+    thus ?thesis unfolding action_over_all_def AND_ALL_iff list_all_iff
+      by simp
+  qed
+
+  have sat_conds: "W \<turnstile> over_all_conds"
+  proof -
+    have "W \<turnstile> action_over_all a" if "a \<in> set action_list" for a
+    proof -
+      from that act_img_actions
+      have "a \<in> actions" by simp
+      thus ?thesis using over_all by simp
+    qed
+    thus ?thesis unfolding over_all_conds_def AND_ALL_iff list_all_iff by simp
+  qed
+  show ?thesis
+    apply (rule steps.step[OF _ steps.refl])
+    apply (rule step_a)
+    apply (rule step_a.intros[where g = over_all_conds])
+    unfolding trans_of_def inv_of_def prob_automaton_def exec_to_main_def 
+    using sat_conds stop by auto
 qed
 
 definition "W\<^sub>0 \<equiv> \<lambda>c. 0"
 
 lemma automaton_complete: "\<exists>W'. \<T> \<turnstile> \<langle>Init, W\<^sub>0\<rangle> \<rightarrow>* \<langle>Goal, W'\<rangle>"
-  sorry
+  sorry               
 end
 
 end
